Prove function transfer triple theorem

Isabelle_Set/Transfer/restructured/Function.thy
@@ -22,6 +22,12 @@ translations
 term "R \<Rrightarrow> S"
 term "[x y \<Colon> R] \<Rrightarrow> S x y"
 
+lemma dep_rel_funE: "\<lbrakk>([x y \<Colon> R] \<Rrightarrow> S x y) f g; R x y\<rbrakk> \<Longrightarrow> S x y (f x) (g y)"
+  unfolding dep_rel_fun_def by blast
+
+lemma dep_rel_funI: "(\<And>x y. R x y \<Longrightarrow> S x y (f x) (g y)) \<Longrightarrow> ([x y \<Colon> R] \<Rrightarrow> S x y) f g"
+  unfolding dep_rel_fun_def by blast
+
 lemma no_dep_rel_funE: "(R \<Rrightarrow> S) f g \<Longrightarrow> R x y \<Longrightarrow> S (f x) (g y)"
   unfolding no_dep_rel_fun_def dep_rel_fun_def
   by blast
@@ -60,7 +66,7 @@ lemma z_property_no_dep_fun_rel:
   using z_propertyE[OF assms(2)]
   by blast
 
-lemma Eq_rep_app:
+lemma Eq_rep_app': (* delete *)
   assumes trans_trip1: "transfer_triple T1 abs1 rep1"
       and trans_trip2: "transfer_triple T2 abs2 rep2"
       and Eq_rep_fun: "Eq_rep (T1 \<Rrightarrow> T2) f f'"
@@ -118,42 +124,263 @@ next
     using h .
 qed
 
-lemma fun_lifting:
-  assumes "transfer_triple T1 abs1 rep1" and "transfer_triple T2 abs2 rep2"
-  shows "transfer_triple (T1 \<Rrightarrow> T2) (map_fun rep1 abs2) (map_fun abs1 rep2)"
+definition dep_map_fun :: "('a \<Rightarrow> 'b) \<Rightarrow> ('b \<Rightarrow> 'c \<Rightarrow> 'd) \<Rightarrow> ('b \<Rightarrow> 'c) \<Rightarrow> 'a \<Rightarrow> 'd"
+  where "dep_map_fun f g h x \<equiv> g (f x) (h (f x))"
+
+(* point-free representation :) *)
+term "S g h y = g y (h y)" (* substitution combinator *)
+term "(S g h \<circ> f) x = S g h (f x) = g (f x) (h (f x))"
+term "dep_map_fun f g h = S g h \<circ> f"
+
+definition map_fun :: "('a \<Rightarrow> 'b) \<Rightarrow> ('c \<Rightarrow> 'd) \<Rightarrow> ('b \<Rightarrow> 'c) \<Rightarrow> 'a \<Rightarrow> 'd"
+  where "map_fun f g h \<equiv> dep_map_fun f (\<lambda>_. g) h"
+
+lemma map_fun_simp: "map_fun f g h \<equiv> g \<circ> h \<circ> f"
+  unfolding map_fun_def dep_map_fun_def comp_def .
+
+lemma Eq_rep_app:
+  assumes trans_trip1: "transfer_triple T1 abs1 rep1"
+      and trans_trip2: "\<And>x y. T1 x y \<Longrightarrow> transfer_triple (T2 x y) (abs2 x) (rep2 y)"
+      and T2_resp: "\<And>x x' y y'. \<lbrakk>T1 x y; Eq_rep T1 x x'; Eq_abs T1 y y'\<rbrakk> \<Longrightarrow> T2 x y = T2 x' y'"
+      and Eq_fun: "Eq_rep (dep_rel_fun T1 T2) f f'"
+      and Eq_arg: "Eq_rep T1 x x'"
+    shows "Eq_rep (T2 x (abs1 x)) (f x) (f' x')"
+proof -
+  obtain g where rel_fun: "dep_rel_fun T1 T2 f g" "dep_rel_fun T1 T2 f' g"
+    using Eq_repE' Eq_fun .
+  obtain y where rel_arg: "T1 x y" "T1 x' y"
+    using Eq_repE' Eq_arg .
+  have Eq_abs_abs_x_y: "Eq_abs T1 (abs1 x) y"
+    using Eq_absI rel_abs trans_trip1 in_domI rel_arg(1, 1) .
+  have rel_res: "T2 x y (f x) (g y)"
+    using dep_rel_funE rel_fun(1) rel_arg(1) .
+  have rel_res': "T2 x' y (f' x') (g y)"
+    using dep_rel_funE rel_fun(2) rel_arg(2) .
+  have Eq_rel1: "T2 x y = T2 x' y"
+    using T2_resp rel_arg(1) Eq_arg Eq_abs_self in_co_domI rel_arg(1) .
+  have Eq_rel2: "T2 x y = T2 x (abs1 x)"
+    using T2_resp rel_arg(1) Eq_rep_self in_domI rel_arg(1) Eq_abs_sym Eq_abs_abs_x_y .
+  show " Eq_rep (T2 x (abs1 x)) (f x) (f' x')"
+    using Eq_repI rel_res[unfolded Eq_rel2] rel_res'[folded Eq_rel1, unfolded Eq_rel2] .
+qed
+
+lemma Eq_abs_app:
+  assumes trans_trip1: "transfer_triple T1 abs1 rep1"
+      and trans_trip2: "\<And>x y. T1 x y \<Longrightarrow> transfer_triple (T2 x y) (abs2 x) (rep2 y)"
+      and T2_resp: "\<And>x x' y y'. \<lbrakk>T1 x y; Eq_rep T1 x x'; Eq_abs T1 y y'\<rbrakk> \<Longrightarrow> T2 x y = T2 x' y'"
+      and Eq_fun: "Eq_abs (dep_rel_fun T1 T2) g g'"
+      and Eq_arg: "Eq_abs T1 y y'"
+    shows "Eq_abs (T2 (rep1 y) y) (g y) (g' y')"
+proof -
+  obtain f where rel_fun: "dep_rel_fun T1 T2 f g" "dep_rel_fun T1 T2 f g'"
+    using Eq_absE' Eq_fun .
+  obtain x where rel_arg: "T1 x y" "T1 x y'"
+    using Eq_absE' Eq_arg .
+  have Eq_rep_x_rep_y: "Eq_rep T1 x (rep1 y)"
+    using Eq_repI rel_arg(1) rel_rep trans_trip1 in_co_domI rel_arg(1) .
+  have rel_res: "T2 x y (f x) (g y)"
+    using dep_rel_funE rel_fun(1) rel_arg(1) .
+  have rel_res': "T2 x y' (f x) (g' y')"
+    using dep_rel_funE rel_fun(2) rel_arg(2) .
+  have Eq_rel1: "T2 x y = T2 x y'"
+    using T2_resp rel_arg(1) Eq_rep_self in_domI rel_arg(1) Eq_arg .
+  have Eq_rel2: "T2 x y = T2 (rep1 y) y"
+    using T2_resp rel_arg(1) Eq_rep_x_rep_y Eq_abs_self in_co_domI rel_arg(1) .
+  show "Eq_abs (T2 (rep1 y) y) (g y) (g' y')"
+    using Eq_absI rel_res[unfolded Eq_rel2] rel_res'[folded Eq_rel1, unfolded Eq_rel2] .
+qed
+
+lemma Eq_rep_abs_transfer_triple:
+  assumes trans_trip: "transfer_triple T abs rep"
+      and Eq_abs: "(Eq_rep T \<Rrightarrow> Eq_abs T) abs abs'"
+      and Eq_rep: "(Eq_abs T \<Rrightarrow> Eq_rep T) rep rep'"
+    shows "transfer_triple T abs' rep'"
 proof (rule transfer_tripleI)
-  show "z_property (T1 \<Rrightarrow> T2)"
-   apply (rule z_property_no_dep_fun_rel)
-     apply (rule z_property_transfer_triple, fact assms)+
-    done
+  show "z_property T"
+    using z_property_transfer_triple trans_trip .
+next
+  fix x
+  assume in_dom_x: "in_dom T x"
+  have 1: "T x (abs x)"
+    using rel_abs trans_trip in_dom_x .
+  have 2: "Eq_abs T (abs x) (abs' x)"
+    using no_dep_rel_funE Eq_abs Eq_rep_self in_dom_x .
+  obtain x' where 3: "T x' (abs x)" "T x' (abs' x)"
+    using Eq_absE' 2 .
+  show "T x (abs' x)"
+    using z_propertyE z_property_transfer_triple trans_trip 1 3 .
+next
+  fix y
+  assume in_co_dom_y: "in_co_dom T y"
+  have 1: "T (rep y) y"
+    using rel_rep trans_trip in_co_dom_y .
+  have 2: "Eq_rep T (rep y) (rep' y)"
+    using no_dep_rel_funE Eq_rep Eq_abs_self in_co_dom_y .
+  obtain y' where 3: "T (rep y) y'" "T (rep' y) y'"
+    using Eq_repE' 2 .
+  show "T (rep' y) y"
+    using z_propertyE z_property_transfer_triple trans_trip 3(2, 1) 1 .
+qed
+
+(* Both, the transfer relation and the abstraction and representation function for the co-domains,
+   may depend on the arguments, however they need to behave in an equivalent way for equivalent
+   arguments. Intuitively, equivalent arguments map to equivalent transfer triples. In particular,
+   this means, that the co-domain relation is fully determined by a single parameter since eg.
+   \<forall>x y. T1 x y \<longrightarrow> T2 x y = T2 x (abs1 x). *)
+lemma fun_transfer_triple:
+  assumes trans_trip1: "transfer_triple T1 abs1 rep1"
+      and trans_trip2: "\<And>x y. T1 x y \<Longrightarrow> transfer_triple (T2 x y) (abs2 x) (rep2 y)"
+      and T2_resp: "\<And>x x' y y'. \<lbrakk>T1 x y; Eq_rep T1 x x'; Eq_abs T1 y y'\<rbrakk> \<Longrightarrow> T2 x y = T2 x' y'"
+      and rep2_resp: "\<And>x y y'. \<lbrakk>T1 x y; Eq_abs T1 y y'\<rbrakk> \<Longrightarrow> (Eq_abs (T2 x y) \<Rrightarrow> Eq_rep (T2 x y)) (rep2 y) (rep2 y')"
+      and abs2_resp: "\<And>x x' y. \<lbrakk>T1 x y; Eq_rep T1 x x'\<rbrakk> \<Longrightarrow> (Eq_rep (T2 x y) \<Rrightarrow> Eq_abs (T2 x y)) (abs2 x) (abs2 x')"
+  shows "transfer_triple (dep_rel_fun T1 T2) (dep_map_fun rep1 abs2) (dep_map_fun abs1 rep2)"
+proof (rule transfer_tripleI)
+  show "z_property (dep_rel_fun T1 T2)"
+  proof (rule z_propertyI, rule dep_rel_funI, (drule dep_rel_funE, assumption)+)
+    fix f1 g1 f2 g2 x y
+    assume rel: "T1 x y"
+       and fun_rels: "T2 x y (f1 x) (g1 y)" "T2 x y (f2 x) (g1 y)" "T2 x y (f2 x) (g2 y)"
+    show "T2 x y (f1 x) (g2 y)"
+      using z_propertyE z_property_transfer_triple assms(2) rel fun_rels .
+  qed
 next
   fix f
-  assume prem1: "in_dom (T1 \<Rrightarrow> T2) f"
-  show "(T1 \<Rrightarrow> T2) f (map_fun rep1 abs2 f)"
-  proof (rule no_dep_rel_funI)
+  assume in_dom_f: "in_dom (dep_rel_fun T1 T2) f"
+  show "dep_rel_fun T1 T2 f (dep_map_fun rep1 abs2 f)"
+  proof (rule dep_rel_funI)
     fix x y
-    assume prem2: "T1 x y"
+    assume rel: "T1 x y"
     have 1: "Eq_rep T1 x (rep1 y)"
-      using Eq_rep_rep[OF assms(1) prem2] .
-    hence "Eq_rep T2 (f x) (f (rep1 y))"
-      using Eq_rep_app[OF assms]
-      using prem1
-      using Eq_repE Eq_repI dep_rel_fun_def in_dom_def no_dep_rel_fun_def prem1
-      sorry
-    show "T2 (f x) (map_fun rep1 abs2 f y)"
-      using assms prem1 prem2
-      using z_propertyE[OF z_property_transfer_triple[OF assms(1)]]
-        z_propertyE[OF z_property_transfer_triple[OF assms(2)]]
-      unfolding in_co_dom_def in_dom_def
-      using no_dep_rel_funE
-      using assms(1) assms(2) in_co_dom_def in_dom_def transfer_triple_def
-      sorry
+      using Eq_rep_rep trans_trip1 rel .
+    have 2: "Eq_abs T1 y (abs1 x)"
+      using Eq_abs_abs trans_trip1 rel .
+    have 3: "T2 x y = T2 x (abs1 x)"
+      using T2_resp rel Eq_rep_self in_domI rel 2 .
+    have 4: "Eq_rep (T2 x y) (f x) (f (rep1 y))"
+      apply (subst 3)
+      apply (rule Eq_rep_app[of T1 _ _ T2])
+      apply (fact trans_trip1 trans_trip2 T2_resp Eq_rep_self[OF in_dom_f] 1)+
+      done
+    have 5: "transfer_triple (T2 x y) (abs2 (rep1 y)) (rep2 y)"
+      using Eq_rep_abs_transfer_triple[OF trans_trip2[OF rel] abs2_resp[OF rel 1]] rep2_resp[OF rel]
+        Eq_abs_self in_co_domI rel .
+    show "T2 x y (f x) (dep_map_fun rep1 abs2 f y)"
+      unfolding dep_map_fun_def
+      using rel_abs' 5 4 .
   qed
 next
   fix g
-  assume prem: "in_co_dom (T1 \<Rrightarrow> T2) g"
-  show "(T1 \<Rrightarrow> T2) (map_fun abs1 rep2 g) g"
-    sorry
+  assume in_co_dom_g: "in_co_dom (dep_rel_fun T1 T2) g"
+  show "dep_rel_fun T1 T2 (dep_map_fun abs1 rep2 g) g"
+  proof (rule dep_rel_funI)
+    fix x y
+    assume rel: "T1 x y"
+    have 1: "Eq_abs T1 y (abs1 x)"
+      using Eq_abs_abs trans_trip1 rel .
+    have 2: "Eq_rep T1 x (rep1 y)"
+      using Eq_rep_rep trans_trip1 rel .
+    have 3: "T2 x y = T2 (rep1 y) y"
+      using T2_resp rel 2 Eq_abs_self in_co_domI rel .
+    have 4: "Eq_abs (T2 x y) (g (abs1 x)) (g y)"
+      apply (subst 3)
+      apply (rule Eq_abs_sym)
+      apply (rule Eq_abs_app[of T1 _ _ T2])
+      apply (fact trans_trip1 trans_trip2 T2_resp Eq_abs_self[OF in_co_dom_g] 1)+
+      done
+    have 5: "transfer_triple (T2 x y) (abs2 x) (rep2 (abs1 x))"
+      using Eq_rep_abs_transfer_triple trans_trip2[OF rel]
+        abs2_resp[OF rel Eq_rep_self[OF in_domI[of T1, OF rel]]]
+        rep2_resp[OF rel 1] .
+    show "T2 x y (dep_map_fun abs1 rep2 g x) (g y)"
+      unfolding dep_map_fun_def
+      using rel_rep' 5 4 .
+  qed
 qed
+
+lemma rel_comp_Eq_abs:
+  assumes trans_trip: "transfer_triple T abs rep"
+  shows "T \<circ>\<circ> Eq_abs T = T"
+proof ((rule ext)+, rule iffI)
+  fix x y
+  assume prem: "(T \<circ>\<circ> Eq_abs T) x y"
+  obtain y' where T_x_y: "T x y'" and Eq_y'_y: "Eq_abs T y' y"
+    using rel_compE prem .
+  obtain x' where T_x'_y': "T x' y'" and T_x'_y: "T x' y"
+    using Eq_absE' Eq_y'_y .
+  show "T x y"
+    using z_propertyE z_property_transfer_triple trans_trip T_x_y T_x'_y' T_x'_y .
+next
+  fix x y
+  assume rel: "T x y"
+  show "(T \<circ>\<circ> Eq_abs T) x y"
+    using rel_compI rel Eq_abs_self in_co_domI rel .
+qed
+
+lemma Eq_rep_rep_comp:
+  assumes trans_trip: "transfer_triple T abs rep"
+  shows "Eq_rep T \<circ>\<circ> T = T"
+proof -
+  have "rel_inv T \<circ>\<circ> Eq_abs (rel_inv T) = rel_inv T"
+    using rel_comp_Eq_abs[OF transfer_triple_dual[OF trans_trip]] .
+  hence "rel_inv T \<circ>\<circ> Eq_rep T = rel_inv T"
+    unfolding Eq_abs_inv_simp .
+  hence "rel_inv T \<circ>\<circ> rel_inv (Eq_rep T) = rel_inv T"
+    apply (subst symmetric_then_eq_rel_inv_self[OF symmetric_Eq_rep]) .
+  hence "rel_inv ((Eq_rep T) \<circ>\<circ> T)  = rel_inv T"
+    unfolding rel_inv_comp_dist .
+  thus "Eq_rep T \<circ>\<circ> T = T"
+    by (rule eq_rel_inv_simp)
+qed
+
+lemma rel_Eq_abs:
+  assumes trans_trip: "transfer_triple T abs rep"
+    and rel: "T x y"
+      and eq: "Eq_abs T y y'"
+    shows "T x y'"
+  apply (subst rel_comp_Eq_abs[OF trans_trip, symmetric])
+  using rel_compI rel eq .
+
+lemma Eq_arg_abs:
+  assumes trans_trip: "transfer_triple T abs rep"
+      and eq: "Eq_rep T x x'"
+    shows "Eq_abs T (abs x) (abs x')"
+proof -
+  obtain y where rels: "T x y" "T x' y"
+    using Eq_repE' eq .
+  have rel_abs1: "T x (abs x)"
+    using rel_abs trans_trip Eq_rep_then_in_dom eq .
+  have rel_abs2: "T x' (abs x')"
+    using rel_abs trans_trip Eq_rep_then_in_dom Eq_rep_sym eq .
+  have  eq_abs1: "Eq_abs T (abs x) y"
+    using Eq_absI rel_abs1 rels(1) .
+  have eq_abs2: "Eq_abs T y (abs x')"
+    using Eq_absI rels(2) rel_abs2 .
+  show "Eq_abs T (abs x) (abs x')"
+    using partial_equivalence_trans partial_equivalnce_Eq_abs z_property_transfer_triple
+      trans_trip eq_abs1 eq_abs2 .
+qed
+
+lemma Eq_arg_rep:
+  assumes trans_trip: "transfer_triple T abs rep"
+      and eq: "Eq_abs T y y'"
+    shows "Eq_rep T (rep y) (rep y')"
+proof -
+  show "Eq_rep T (rep y) (rep y')"
+    apply (subst Eq_abs_inv_simp[symmetric])
+    using Eq_arg_abs transfer_triple_dual[OF trans_trip] eq[folded Eq_rep_inv_simp] .
+qed
+
+lemma no_dep_fun_transfer_triple:
+  assumes trans_trip1: "transfer_triple T1 abs1 rep1"
+      and trans_trip2: "transfer_triple T2 abs2 rep2"
+    shows "transfer_triple (T1 \<Rrightarrow> T2) (map_fun rep1 abs2) (map_fun abs1 rep2)"
+  unfolding no_dep_rel_fun_def map_fun_def
+  apply (rule fun_transfer_triple)
+  apply (rule trans_trip1 trans_trip2 refl)+
+   apply (rule no_dep_rel_funI)
+  apply (rule Eq_arg_rep[OF trans_trip2], assumption)
+   apply (rule no_dep_rel_funI)
+  apply (rule Eq_arg_abs[OF trans_trip2], assumption)
+  done
 
 end
